cryptis/lib/list_sort.v
@@ -1,0 +1,60 @@
+(** Small generic list utilities on top of stdpp, used to canonicalise lists
+    with [merge_sort]:
+
+    - [rem x l] removes the *first* occurrence of [x] from [l] (like mathcomp's
+      [seq.rem]), parameterised by an [EqDecision] instance.  stdpp has no
+      first-occurrence removal (its [list_difference] removes *all* matches, and
+      the multiset view [elem_of_Permutation] is only existential), so we define
+      it here.
+
+    - lemmas relating [merge_sort R] (for an arbitrary decidable total order [R])
+      to membership, [Forall], length and sortedness. *)
+
+From mathcomp Require Import ssreflect.
+From stdpp Require Import sorting list.
+
+Section Rem.
+Context {A : Type} `{EqDecision A}.
+Implicit Types (x z : A) (l : list A).
+
+Fixpoint rem x l : list A :=
+  match l with
+  | [] => []
+  | y :: l => if bool_decide (x = y) then l else y :: rem x l
+  end.
+
+Lemma elem_of_rem {z x l} : z ∈ rem x l -> z ∈ l.
+Proof.
+elim: l => [|a l IH] //=.
+case_bool_decide as H.
+- move=> ?; exact: list_elem_of_further.
+- rewrite !elem_of_cons; move=> [->|/IH ?]; by [left|right].
+Qed.
+
+End Rem.
+
+Section MergeSort.
+Context {A : Type} (R : relation A)
+  `{!RelDecision R, !Transitive R, !Total R, !AntiSymm (=@{A}) R}.
+Implicit Types (x : A) (l : list A) (P : A -> Prop).
+
+Lemma elem_of_merge_sort x l : x ∈ merge_sort R l ↔ x ∈ l.
+Proof. by rewrite (merge_sort_Permutation R l). Qed.
+
+Lemma Forall_merge_sort P l : Forall P (merge_sort R l) ↔ Forall P l.
+Proof. by rewrite (merge_sort_Permutation R l). Qed.
+
+Lemma length_merge_sort l : length (merge_sort R l) = length l.
+Proof. by rewrite (merge_sort_Permutation R l). Qed.
+
+Lemma merge_sort_sorted l : StronglySorted R (merge_sort R l).
+Proof. apply: StronglySorted_merge_sort. Qed.
+
+Lemma merge_sort_id l : StronglySorted R l -> merge_sort R l = l.
+Proof.
+move=> H.
+exact: (StronglySorted_unique R (merge_sort R l) l
+          (merge_sort_sorted l) H (merge_sort_Permutation R l)).
+Qed.
+
+End MergeSort.
